More work in Pred.v

src/Pred.v
@@ -1,5 +1,6 @@
 Require Import
   Coq.ZArith.ZArith
+  Coq.Logic.PropExtensionality
   Hask.Control.Monad
   Hask.Data.Either
   Pact.ilist
@@ -12,7 +13,10 @@ Require Import
   Pact.SemTy
   Pact.Lang
   Pact.Lang.Capability
-  Pact.SemExp.
+  Pact.SemExp
+  Coq.Classes.RelationClasses
+  Coq.Classes.Morphisms
+  Pact.Ltac.
 
 Set Implicit Arguments.
 Unset Strict Implicit.
@@ -29,63 +33,306 @@ Section Pred.
 
 Definition env   : Type := PactEnv.
 Definition state : Type := PactState.
-Definition log   : Type := PactLog.
 
-(* Definition EvalP (r : env) (s : state) `(e : Exp [] τ) *)
-(*   (s' : state) (v : SemTy τ) (er : Err) : Prop := *)
+Definition rprop   : Type := env → Prop.
+Definition sprop   : Type := state → Prop.
+Definition eprop   : Type := Err → Prop.
+Definition vprop τ : Type := SemTy (m:=PactM) τ → sprop.
 
-Implicit Type G : env → Prop.
-Implicit Type H : state → Prop.
-Implicit Type Z : Err → Prop.
+Implicit Type G : rprop.
+Implicit Type H : sprop.
+Implicit Type Z : eprop.
 
-Definition hoare
-  (G : env → Prop)
-  (H : state → Prop)
-  `(e : Exp [] τ)
-  (Q : ⟦τ⟧ → state → Prop)
-  (Y : log → Prop)
-  (Z : Err → Prop) : Prop :=
+Definition hoare G H `(e : Exp [] τ) (Q : vprop τ) Z : Prop :=
   ∀ (r : env), G r →
   ∀ (s : state), H s ->
-  match ⟦e⟧ r s : Err + ⟦τ⟧ * (state * log) with
-  | inr (v, (s', w)) => Q v s' ∧ Y w
+  match ⟦e⟧ r s : Err + ⟦τ⟧ * (state * _) with
+  | inr (v, (s', _)) => Q v s'
   | inl err => Z err
   end.
 
-Notation "{ G & H } x ← e { Q & Y | Z }" :=
-  (hoare G H e (λ x, Q) Y Z) (at level 1, e at next level).
+Declare Scope pred_scope.
+Open Scope pred_scope.
+
+Notation "{ G & H } x ← e { Q | Z }" :=
+  (hoare G H e (λ x, Q) Z) (at level 1, e at next level) : pred_scope.
 
 #[local] Hint Unfold hoare : core.
 
-Theorem hoare_post_true G H `(Q : ⟦τ⟧ → state → Prop) (Y : log → Prop) Z e :
+Theorem hoare_post_true G H `(Q : vprop τ) Z e :
   (∀ v s, Q v s) →
-  (∀ l, Y l) →
   (∀ err, Z err) →
-  { G & H } x ← e { Q x & Y | Z }.
+  { G & H } x ← e { Q x | Z }.
 Proof.
   unfold hoare; sauto.
 Qed.
 
-Theorem hoare_pre_false G H `(Q : ⟦τ⟧ → state → Prop) (Y : log → Prop) Z e :
+Theorem hoare_pre_false G H `(Q : vprop τ) Z e :
   (∀ r, ¬ (G r)) ∨ (∀ s, ¬ (H s)) →
-  { G & H } x ← e { Q x & Y | Z }.
+  { G & H } x ← e { Q x | Z }.
 Proof.
   unfold hoare; sauto.
 Qed.
 
-Definition hprop_conj `(Q : state → Prop) (H : state → Prop) : state → Prop :=
-  λ st, Q st ∧ H st.
+Definition sprop_conj (H H' : sprop) : sprop :=
+  λ st, H st ∧ H' st.
 
-Notation "Q \∧ H" := (hprop_conj Q H) (at level 10).
+Arguments sprop_conj _ _ /.
+
+#[local] Hint Unfold sprop_conj : core.
+
+Notation "Q \∧ H" := (sprop_conj Q H) (at level 10) : pred_scope.
 
 Definition quadruple
-  (G : env → Prop)
-  (H : state → Prop)
+  (G : rprop)
+  (H : sprop)
   `(e : Exp [] τ)
-  (Q : ⟦τ⟧ → state → Prop)
-  (Y : log → Prop)
-  (Z : Err → Prop) : Prop :=
-  ∀ H', { G & H \∧ H' } x ← e { Q x \∧ H' & Y | Z }.
+  (Q : vprop τ)
+  (Z : eprop) : Prop :=
+  ∀ H', { G & H \∧ H' } x ← e { Q x \∧ H' | Z }.
+
+#[local] Hint Unfold quadruple : core.
+
+Theorem frame_rule {G H} `{e : Exp [] τ} {Q Z H'} :
+  quadruple G H e Q Z →
+  quadruple G (H \∧ H') e (λ x, Q x \∧ H') Z.
+Proof.
+  unfold quadruple, hoare.
+  intros.
+  destruct H2, H2.
+  pose proof (H0 _ _ H1 _ (conj H2 H4)).
+  pose proof (H0 _ _ H1 _ (conj H2 H3)).
+  sauto lq: on.
+Qed.
+
+Definition WP : Type :=
+  ∀ τ (e : Exp [] τ) (Q : vprop τ) (Z : eprop), env → sprop.
+
+Definition wp
+  `(e : Exp [] τ)
+  (Q : vprop τ)
+  (Z : eprop) : env → sprop :=
+  λ r st,
+    ∃ (G : rprop) (H : sprop),
+      G r ∧ (H \∧ (λ _, quadruple G H e Q Z) st).
+
+#[local] Hint Unfold wp : core.
+
+Definition himpl (P Q : sprop) : Prop :=
+  ∀ s, P s → Q s.
+
+#[local] Hint Unfold himpl : core.
+
+Notation "P ==> Q" :=
+  (himpl P Q) (at level 55, Q at level 55) : pred_scope.
+
+Definition hrimpl (G : rprop) (P : sprop) (Q : env → sprop) : Prop :=
+  ∀ r s, G r → P s → Q r s.
+
+#[local] Hint Unfold hrimpl : core.
+
+Notation "P =[ G ]=> Q" :=
+  (hrimpl G P Q) (at level 55, G at level 55, Q at level 55) : pred_scope.
+
+Lemma dehrimpl `(H : P =[ G ]=> Q) : ∀ r, G r → P ==> Q r.
+Proof.
+  unfold himpl, hrimpl in *.
+  intuition.
+Defined.
+
+Lemma hrimplize `(H : ∀ r, G r → P ==> Q r) : P =[ G ]=> Q.
+Proof.
+  unfold himpl, hrimpl in *.
+  intuition.
+Defined.
+
+Corollary dehrimpl_hrimplize `(H : ∀ r, G r → P ==> Q r) :
+  dehrimpl (hrimplize H) = H.
+Proof. reflexivity. Qed.
+
+Corollary hrimplize_dehrimpl `(H : P =[ G ]=> Q) :
+  hrimplize (dehrimpl H) = H.
+Proof. reflexivity. Qed.
+
+Definition qimpl {τ} (Q R : vprop τ) : Prop :=
+  ∀ v, Q v ==> R v.
+
+#[local] Hint Unfold qimpl : core.
+
+Notation "Q ===> R" := (qimpl Q R) (at level 55) : pred_scope.
+
+Theorem wp_equiv {G H} `{e : Exp [] τ} {Q Z} :
+  (H =[G]=> wp e Q Z) ↔ (quadruple G H e Q Z).
+Proof.
+  unfold hrimpl, wp, quadruple, hoare, sprop_conj.
+  split; intros.
+  - reduce.
+    specialize (H0 _ _ H1 H2).
+    reduce.
+    unshelve epose proof (H5 _ r _ s (conj _ H3)); auto.
+  - exists G.
+    exists H.
+    split; auto.
+Qed.
+
+Lemma pred_ext_1 (A1 : Type) :
+  ∀ (P Q : ∀ (x1 : A1), Prop),
+    (forall x1, P x1 <-> Q x1) -> P = Q.
+Proof.
+  intros.
+  extensionality x.
+  now apply propositional_extensionality.
+Qed.
+
+Lemma himpl_refl {H} :
+  H ==> H.
+Proof. now repeat intro. Qed.
+
+Lemma himpl_trans {H1 H2 H3} :
+  (H1 ==> H2) →
+  (H2 ==> H3) →
+  (H1 ==> H3).
+Proof.
+  repeat intro.
+  unfold himpl in *.
+  intuition.
+Qed.
+
+#[export]
+Program Instance himpl_PreOrder : PreOrder himpl.
+
+Lemma himpl_antisym {H1 H2} :
+  (H1 ==> H2) →
+  (H2 ==> H1) →
+  (H1 = H2).
+Proof.
+  unfold himpl.
+  intros.
+  apply pred_ext_1.
+  sauto.
+Qed.
+
+Theorem wp_unique (wp1 wp2 : WP) :
+  (∀ G H τ (e : Exp [] τ) Q Z,
+     quadruple G H e Q Z ↔ H =[G]=> wp1 _ e Q Z) →
+  (∀ G H τ (e : Exp [] τ) Q Z,
+     quadruple G H e Q Z ↔ H =[G]=> wp2 _ e Q Z) →
+  wp1 = wp2.
+Proof.
+  intros.
+  extensionality τ.
+  extensionality e.
+  extensionality Q.
+  extensionality Z.
+  extensionality r.
+  apply himpl_antisym.
+  - destruct (H0 (λ r', r = r') (wp1 τ e Q Z r) τ e Q Z) as [H5 H6]; clear H0.
+    eapply dehrimpl in H5; eauto.
+    apply H; intros.
+    subst.
+    apply hrimplize; intros; subst.
+    apply himpl_refl.
+  - destruct (H (λ r', r = r') (wp2 τ e Q Z r) τ e Q Z) as [H5 H6]; clear H.
+    eapply dehrimpl in H5; eauto.
+    apply H0; intros.
+    subst.
+    apply hrimplize; intros; subst.
+    apply himpl_refl.
+Qed.
+
+Theorem triple_conseq {G τ} {e : Exp [] τ} {H' Q' H Q Z} :
+  quadruple G H' e Q' Z →
+  H ==> H' →
+  Q' ===> Q →
+  quadruple G H e Q Z.
+Proof.
+  intros.
+  repeat intro.
+  destruct H4.
+  specialize (H1 _ H4).
+  specialize (H0 H'0 _ H3 _ (conj H1 H5)).
+  matches.
+  reduce.
+  unfold sprop_conj in *.
+  intuition.
+Qed.
+
+Lemma vimpl_refl {τ} {Q : vprop τ} :
+  Q ===> Q.
+Proof. now repeat intro. Qed.
+
+Theorem wp_from_weakest_pre (wp' : WP) :
+  (∀ G H τ (e : Exp [] τ) Q Z r,
+     quadruple G (wp' _ e Q Z r) e Q Z) →          (* wp_pre *)
+  (∀ G H τ (e : Exp [] τ) Q Z,
+     quadruple G H e Q Z → ∀ r, G r → H ==> wp' _ e Q Z r) → (* wp_weakest *)
+  (∀ G H τ (e : Exp [] τ) Q Z,
+     ∀ r, G r → H ==> wp' _ e Q Z r ↔ quadruple G H e Q Z).  (* wp_equiv *)
+Proof.
+  intros M1 M2.
+  split; intro M.
+  - eapply triple_conseq; eauto.
+  - eapply M2; eauto.
+Qed.
+
+#[local] Hint Unfold RWSE_join : core.
+#[local] Hint Unfold RWSE_ap : core.
+#[local] Hint Unfold Either_map : core.
+#[local] Hint Unfold Tuple.first : core.
+#[local] Hint Unfold Basics.compose : core.
+#[local] Hint Unfold Datatypes.id : core.
+
+Notation "G =====> H" :=
+  (∀ Q Z r, wp G Q Z r ==> wp H Q Z r) (at level 100, H at next level) : pred_scope.
+
+Lemma quadruple_if G H b τ (t1 t2 : Exp [] τ) Q Z :
+  quadruple G H (if b then t1 else t2) Q Z →
+  quadruple G H (If (Lit (LitBool b)) t1 t2) Q Z.
+Proof.
+  autounfold.
+  repeat intro.
+  reduce.
+  simp SemExp; simpl.
+  autounfold.
+  specialize (H0 _ _ H1 _ (conj H2 H3)).
+  destruct b; sauto.
+Qed.
+
+(* An if statement simply propagates the environment. *)
+Lemma wp_if b τ (t1 t2 : Exp [] τ) :
+  (if b then t1 else t2) =====> If (Lit (LitBool b)) t1 t2.
+Proof.
+  intros.
+  apply (dehrimpl (G:=λ r', r = r')); eauto.
+  eapply wp_equiv.
+  apply quadruple_if.
+  eapply wp_equiv.
+  apply hrimplize; intros.
+  subst.
+  reflexivity.
+Qed.
+
+Lemma quadruple_app_fun G H `(v : Exp [] dom) `(e : Exp [dom] cod) Q Z :
+  ValueP v →
+  quadruple G H (SubExp {|| v ||} e) Q Z →
+  quadruple G H (APP (LAM e) v) Q Z.
+Proof.
+  autounfold.
+  simp SemExp; simpl.
+  autounfold.
+  intros.
+  specialize (H1 _ _ H2 _ H3).
+  autounfold.
+  pose proof (SemExp_ValueP (Γ:=[]) tt H0).
+  reduce.
+  rewrite H4; simpl.
+  rewrite NoSub_idSub in H1.
+  erewrite SemExp_SubExp in H1; eauto.
+  simpl in *.
+  destruct (⟦ (x, ()) ⊨ e ⟧ r s); auto.
+  reduce.
+  intuition.
+Qed.
 
 (* This encodes a boolean predicate in positive normal form. *)
 Inductive Pred Γ : ∀ {τ}, Γ ⊢ τ → Set :=
